\subsection{Zadanie 8}

$L(x,m,\sigma)=\displaystyle\prod\limits_{i=1}^n f_{m,\sigma} (x_i)$ - funkcja niepewno≈õci

$$l=ln L(x,m,\sigma)=ln \displaystyle\prod\limits_{i=1}^n f_{m,\sigma} (x_i)=\displaystyle\sum\limits_{i=1}^n ln(f_{m,\sigma} (x_i))$$

$$l(x)=\displaystyle\sum\limits_{i=1}^n ln(\frac{1}{\sqrt{2\pi\sigma^2}}e^{-\frac{(x-m)^2}{2\sigma^2}})=\displaystyle\sum\limits_{i=1}^n ln (\frac{1}{\sqrt{2\pi\sigma^2}})+\displaystyle\sum\limits_{i=1}^n e^{-\frac{(x-m)^2}{2\sigma^2}}=\displaystyle\sum\limits_{i=1}^n ln (\frac{1}{\sqrt{2\pi\sigma^2}})+\displaystyle\sum\limits_{i=1}^n {\frac{(x-m)^2}{\sigma^2}}$$

$${\frac{\theta}{\theta m}}L(x_i,m_i,\sigma)=\displaystyle\sum\limits_{i=1}^n 2{\frac{(x_i-m)^2}{2\sigma^2}}={\frac{1}{\sigma^2}}(\displaystyle\sum\limits_{i=1}^n x_i-nm)$$

$${\frac{1}{\sigma^2}}(\displaystyle\sum\limits_{i=1}^n x_i-nm)=0 \Leftrightarrow\displaystyle\sum\limits_{i=1}^n x_i-nm=0$$

$$\displaystyle\sum\limits_{i=1}^n x_i=nm$$

$$m={\frac{\displaystyle\sum\limits_{i=1}^n x_i}{n}}$$
